Support dynamic offsets in wp_load_gc

theories/iris/gc.v
@@ -51,8 +51,14 @@ Inductive repr_vblock : addr_map -> vblock -> list i32 -> Prop :=
       Forall (curry (repr_vval θ)) (combine blk.(vals) ks) ->
       repr_vblock θ blk ks.
 
-Definition vblock_offset (i : nat) : static_offset :=
-  N.of_nat (4 * i).
+Definition vblock_offset (i : nat) : N := N.of_nat (4 * i).
+
+Inductive repr_vloc_offset : addr_map -> vloc -> nat -> i32 -> Prop :=
+  | RVloc_offset θ ℓ i a a' :
+      θ !! ℓ = Some a ->
+      a' = (a + vblock_offset i)%N ->
+      (Z.of_N a' < Wasm_int.Int32.modulus)%Z ->
+      repr_vloc_offset θ ℓ i (code_addr a').
 
 Definition roots_are_live (θ : addr_map) (roots : gmap addr vval) : Prop :=
   ∀ a ℓ, roots !! a = Some (Vloc ℓ) -> ℓ ∈ dom θ.
@@ -122,13 +128,13 @@ Lemma list_pluck : forall (A : Type) i (l : list A),
   exists l1 x l2, l !! i = Some x /\ length l1 = i /\ l = l1 ++ x :: l2.
 Admitted.
 
-Lemma repr_vblock_index_word : forall θ blk u ws i,
+Lemma repr_vblock_index : forall θ blk u ks i,
   blk.(vals) !! i = Some u ->
-  repr_vblock θ blk ws ->
-  exists w, repr_vval θ u w /\ ws !! i = Some w.
+  repr_vblock θ blk ks ->
+  exists w, repr_vval θ u w /\ ks !! i = Some w.
 Proof.
-  intros θ blk u ws i Hi Hblk. inversion Hblk. subst.
-  assert (exists w, In (u, w) (combine (vals blk) ws)).
+  intros θ blk u ks i Hi Hblk. inversion Hblk. subst.
+  assert (exists w, In (u, w) (combine (vals blk) ks)).
   - admit.
   - destruct H3 as [w Hw].
     exists w. split.
@@ -158,36 +164,36 @@ Qed.
 Lemma wp_load_gc
     (s : stuckness) (E : coPset) (m : memaddr) (θ : addr_map)
     (i : i32) (ℓ : vloc) (blk : vblock)
-    (j : nat) (off : static_offset) (vv : vval)
+    (off1 off2 : nat) (off2b : static_offset) (vv : vval)
     (F : frame) :
   F.(f_inst).(inst_memory) !! 0 = Some m ->
-  repr_vval θ (Vloc ℓ) i ->
-  blk.(vals) !! j = Some vv ->
-  vblock_offset j = off ->
+  repr_vloc_offset θ ℓ off1 i ->
+  blk.(vals) !! (off1 + off2) = Some vv ->
+  vblock_offset off2 = off2b ->
   GC m θ ∗ ℓ ↦vblk blk ∗ ↪[frame] F ⊢
-  WP [AI_basic (BI_const (VAL_int32 i)); AI_basic (BI_load T_i32 None N.zero off)]
+  WP [AI_basic (BI_const (VAL_int32 i)); AI_basic (BI_load T_i32 None N.zero off2b)]
      @ s; E
      {{ w, (∃ k, ⌜w = immV [VAL_int32 k]⌝ ∗ ⌜repr_vval θ vv k⌝) ∗
            GC m θ ∗ ℓ ↦vblk blk ∗ ↪[frame] F }}.
 Proof.
   iIntros (Em Hk Eu Hoff) "(HGC & Hℓ & HF)".
   iDestruct "HGC" as (ζ roots) "(Hζ & Hroots & Hζmem & Hrootsmem & %Hlive & %GCOK)".
-  inversion Hk as [|θ' ℓ' a Eθℓ Ha32 Eθ' Eℓ' Ek]. subst.
+  inversion Hk as [θ' ℓ' off1' a a' Eθℓ Ea' Ha32 Eθ' Eℓ' Eoff1' Ei]. subst.
   iDestruct (ghost_map_lookup with "Hζ Hℓ") as "%Eζℓ".
   iDestruct (big_sepM2_lookup_acc _ _ _ _ _ _ Eθℓ Eζℓ with "Hζmem") as "[(%bs & %ws & Ha & %Hbs & %Hws) Hζmem]".
   inversion Hws as [θ' blk' vbs Hwslen Hvals Evbs Eθ' Ews]. subst.
   pose proof (lookup_lt_Some _ _ _ Eu) as Hilt. rewrite <- Hwslen in Hilt.
   destruct (list_pluck _ _ _ Hilt) as [ws1 [wsi [ws2 [Hwsi [Hws1len Ews]]]]]. rewrite Ews.
   (* wsi = w *)
-  destruct (repr_vblock_index_word θ blk vv ws j Eu Hws) as [w [Huw Hwi]].
+  destruct (repr_vblock_index θ blk vv ws (off1 + off2) Eu Hws) as [w [Huw Hwi]].
   assert (w = wsi) by congruence. subst wsi.
   unfold serialize_i32s.
   rewrite flat_map_app. rewrite (separate1 w). rewrite flat_map_app. simpl. rewrite app_nil_r.
-  rewrite (wms_app _ _ _ (vblock_offset j)). rewrite (wms_app _ (serialise_i32 w) _ 4).
+  rewrite (wms_app _ _ _ (vblock_offset (off1 + off2))). rewrite (wms_app _ (serialise_i32 w) _ 4).
   iDestruct "Ha" as "(Ha1 & Hai & Ha2)".
   (* add the loaded wms into the postcondition *)
   iApply (wp_wand _ _ _ (λ w0, ((∃ w', ⌜w0 = immV [VAL_int32 w']⌝ ∗ ⌜repr_vval θ vv w'⌝) ∗
-                               N.of_nat m ↦[wms][Wasm_int.N_of_uint i32m (code_addr a) + vblock_offset j] serialise_i32 w) ∗
+  N.of_nat m ↦[wms][Wasm_int.N_of_uint i32m (code_addr (a + vblock_offset off1)) + vblock_offset off2] serialise_i32 w) ∗
                                ↪[frame] F)%I
           with "[HF Hai] [Hζ Hroots Hrootsmem Hℓ Ha1 Ha2 Hζmem]").
   - iApply wp_load_deserialize.
@@ -195,11 +201,13 @@ Proof.
     + assumption.
     + unfold code_addr. rewrite deserialise_serialise_i32. cbn.
       rewrite Wasm_int.Int32.Z_mod_modulus_id.
-      * rewrite N2Z.id. iFrame. by iExists w.
+      * rewrite N2Z.id. replace (vblock_offset (off1 + off2)) with ((vblock_offset off1 + vblock_offset off2)%N).
+        -- rewrite N.add_assoc. iFrame. by iExists w.
+        -- unfold vblock_offset. lia.
       * lia.
   - iIntros (v) "[[HΦ Hai] HF]". iFrame "∗ %". iCombine "Ha1 Hai" as "Ha1".
     unfold code_addr. cbn. rewrite Wasm_int.Int32.Z_mod_modulus_id; last lia. rewrite N2Z.id.
-    rewrite <- wms_app; last first.
+    rewrite <- (N.add_assoc _ (vblock_offset off1) _). rewrite <- wms_app; last first.
     { rewrite (@flat_map_constant_length _ _ 4).
       - rewrite Hws1len. unfold vblock_offset. lia.
       - intros x Hx. unfold serialise_i32. rewrite Memdata.encode_int_length. reflexivity. }
